Definining [administrative_instruction_rect'].

theories/wasm.v
@@ -468,11 +468,52 @@ Definition upd_s_mem (s : store_record) (m : list mem) : store_record :=
     (s_globs s).
 
 Inductive administrative_instruction : Type := (* e *)
-| Basic : basic_instruction -> administrative_instruction
-| Trap
-| Callcl : function_closure -> administrative_instruction
-| Label : nat -> list administrative_instruction -> list administrative_instruction -> administrative_instruction
-| Local : nat -> instance -> list value -> list administrative_instruction -> administrative_instruction.
+  | Basic : basic_instruction -> administrative_instruction
+  | Trap
+  | Callcl : function_closure -> administrative_instruction
+  | Label : nat -> seq administrative_instruction -> seq administrative_instruction -> administrative_instruction
+  | Local : nat -> instance -> list value -> seq administrative_instruction -> administrative_instruction.
+
+(** Induction scheme for [administrative_instruction]. **)
+Section administrative_instruction_rect'.
+
+  Inductive Forall (A : Type) (P : A -> Type) : seq A -> Type :=
+    | Forall_nil : Forall P nil
+    | Forall_cons : forall e l, P e -> Forall P l -> Forall P (e :: l)
+  .
+
+  Variable P : administrative_instruction -> Type.
+
+  Hypothesis basic : forall b, P (Basic b).
+  Hypothesis trap : P Trap.
+  Hypothesis callcl : forall f, P (Callcl f).
+  Hypothesis label : forall n es1 es2,
+    Forall P es1 ->
+    Forall P es2 ->
+    P (Label n es1 es2).
+  Hypothesis local : forall n i vs es,
+    Forall P es ->
+    P (Local n i vs es).
+
+  Fixpoint administrative_instruction_rect' e : P e :=
+    let rect_list :=
+      fix rect_list es : Forall P es :=
+        match es with
+        | [::] => Forall_nil _
+        | e :: l => Forall_cons (administrative_instruction_rect' e) (rect_list l)
+        end in
+    match e with
+    | Basic b => basic b
+    | Trap => trap
+    | Callcl f => callcl f
+    | Label n es1 es2 => label n (rect_list es1) (rect_list es2)
+    | Local n i vs es => local n i vs (rect_list es)
+    end.
+
+End administrative_instruction_rect'.
+
+Definition administrative_instruction_ind' (P : administrative_instruction -> Prop) :=
+  @administrative_instruction_rect' P.
 
 Fixpoint administrative_instruction_eqb (e1 e2 : administrative_instruction) : bool :=
   let fff :=
@@ -497,13 +538,71 @@ Fixpoint administrative_instruction_eqb (e1 e2 : administrative_instruction) : b
     (instance_eqb i1 i2) &&
     (vs1 == vs2) &&
     (fff es1 es2)
-  | _, _ => (* TODO *) false
+  | _, _ => false
   end.
 
-Parameter eqadministrative_instructionP : Equality.axiom administrative_instruction_eqb.
-(* TODO *)
+Lemma eqadministrative_instructionP : Equality.axiom administrative_instruction_eqb.
+Proof.
+  assert (IH: forall es es',
+    Forall (fun x => forall y, reflect (x = y) (administrative_instruction_eqb x y)) es ->
+    reflect (es = es')
+      ((fix f (l1 l2 : list administrative_instruction) :=
+         match l1, l2 with
+         | nil, nil => true
+         | cons _ _, nil => false
+         | nil, cons _ _ => false
+         | cons x xs, cons y ys => (administrative_instruction_eqb x y) && (f xs ys)
+         end) es es')).
+  { elim.
+    - case.
+      + move=> IH. by apply ReflectT.
+      + move=> a l IH. by apply ReflectF.
+    - move=> a l IH. case.
+      + move=> IH'. by apply ReflectF.
+      + move=> a' l' IH'. inversion_clear IH' as [|? ? IH1 IH2].
+        eapply iffP; first by apply andP.
+        * case => ? ?. f_equal.
+          -- by apply/IH1.
+          -- by apply/IH.
+        * case=> ? ?. split.
+          -- by apply/IH1.
+          -- by apply/IH.
+  }
+  move=> x. induction x using administrative_instruction_rect';
+    move=> y; destruct y; simpl;
+    try (apply ReflectF; discriminate).
+  - eapply iffP; first by apply/eqP.
+    + by elim.
+    + by case.
+  - by apply ReflectT.
+  - eapply iffP; first by apply/eqP.
+    + by elim.
+    + by case.
+  - apply iffP with (P := n = n0 /\ es1 = l /\ es2 = l0).
+    + move: (IH es1 l X) (IH es2 l0 X0) => {IH X X0} R1 R2.
+      eapply iffP; first by apply andP.
+      * case. move/andP. case=> ? ? ?. split; first by apply/eqP.
+        split; first by apply/R1. by apply/R2.
+      * intros (?&?&?). subst. split; last by apply/R2.
+        apply/andP. split; last by apply/R1. by apply/eqP.
+    + by repeat (case; elim).
+    + by case.
+  - apply iffP with (P := n = n0 /\ i = i0 /\ vs = l /\ es = l0).
+    + move: (IH es l0 X) => {IH X} R.
+      eapply iffP; first by apply andP.
+      * case. move/andP. case. move/andP. case=> ? ? ? ?.
+        repeat (split; first by apply/eqP). by apply/R.
+      * intros (?&?&?&?). subst. split; last by apply/R.
+        apply/andP. split; last by apply/eqP.
+        apply/andP. split; first by apply/eqP.
+        by apply/eqinstanceP.
+    + by repeat (case; elim).
+    + by case.
+Qed.
+
 Canonical Structure administrative_instruction_eqMixin := EqMixin eqadministrative_instructionP.
-Canonical Structure administrative_instruction_eqType := Eval hnf in EqType administrative_instruction administrative_instruction_eqMixin.
+Canonical Structure administrative_instruction_eqType :=
+  Eval hnf in EqType administrative_instruction administrative_instruction_eqMixin.
 
 
 Inductive lholed : Type :=
